\documentclass[12pt, letterpaper, oneside]{book}
\usepackage{amsmath}
\usepackage{amssymb}
\usepackage{empheq}
\usepackage[letterpaper, textwidth=7.5in, textheight=8in]{geometry}
\usepackage{csquotes}
\usepackage{parskip}

\title{Exercises in \textit{Basic Analysis I: Introduction to Real Analysis, Volume 1}}
\author{Yaobin Wen}
\date{Jan 2024}

\begin{document}

\maketitle
\tableofcontents

% =============================================================================
%
% Chapter 1: Real Numbers
%
% =============================================================================

\chapter{Real Numbers}

% =============================================================================
\section{Exercises 1.1.1}
% =============================================================================

% ******************************
\subsection{Exercise 1.1.1}
% ******************************

\textbf{Proof}: This exercise requires to prove part (iii) of Proposition 1.1.8. That means I can make use of part (i)
and part (ii) in Proposition 1.1.8. The proof steps are as follows:
\begin{itemize}
  \item (a) $\because x < 0, \therefore (-x) > 0, \therefore (-x)y < (-x)z$ (Proposition 1.1.8 (i), (ii))
  \item (b) $\because (-x)y < (-x)z, \therefore (-x)y + xy < (-x)z + xy$ (Definition 1.1.7 (i))
  \item (c) $(-x)y + xy = (-x + x)y = 0y = 0$ (Definition 1.1.5 (D), (A5), (A2))
  \item (d) $\therefore 0 < (-x)z + xy$. ((b), (c))
  \item (e) $\therefore 0 + xz < (-x)z + xy + xz$ (Definition 1.1.7 (i))
  \item (f) $0 + xz = xz$ (Definition 1.1.5 (A4))
  \item (g) $(-x)z + xy + xz = \left((-x)z + xy\right) + xz = \left(xy + (-x)z\right) + xz =
          xy + \left((-x)z + xz \right) = xy + \left((-x) + x\right)z = xy + 0z = xy + 0 = xy$ (Definition 1.1.5 (D),
        (A2), (A3), (A4))
  \item (h) $\therefore xz < xy; \therefore xy > xz$ ((f), (g))
\end{itemize}

\end{document}
