% Regarding `oneside` (https://stackoverflow.com/a/8371473/630364):
%
% `oneside` removes the blank pages between chapters.
% "Note that this method make the margins of all the pages the same. In
% `twoside`, the margins are different for the odd and the even pages".
\documentclass[12pt, letterpaper, oneside]{book}
\usepackage{amsfonts}
\usepackage{amsmath}
\usepackage{amssymb}
\usepackage{csquotes}
\usepackage{float}
\usepackage{hyperref}
\usepackage[letterpaper, textwidth=7.5in, textheight=8in]{geometry}
\hypersetup{
  colorlinks=true,
  linkcolor=blue,
  filecolor=magenta,
  urlcolor=blue,
}
\usepackage{parskip}

\title{
  Notes on \textit{Basic Analysis I: Introduction to Real Analysis, Volume 1}
}
\author{Yaobin Wen}
\date{July 2023}

\begin{document}

\maketitle
\tableofcontents

\chapter*{Overview}
\addcontentsline{toc}{chapter}{Overview}

This document contains my study notes of the textbook \textit{Basic Analysis I:
Introduction to Real Analysis, Volume 1}. I use it for a few purposes:

\begin{enumerate}
  \item As a reference to quickly refresh my memory on the subjects.
  \item Keep the notes to help me understand the text that is not obvious for
    me to comprehend.
\end{enumerate}

% =============================================================================
%
% Chapter: Review of Real Numbers
%
% =============================================================================

\chapter*{Introduction}
\addcontentsline{toc}{chapter}{Introduction}

% =============================================================================
\section{About this book}
% =============================================================================

(Nothing to write down.)

% =============================================================================
\section{About analysis}
% =============================================================================

The \textbf{most important difference} between analysis and algebra:
\begin{itemize}
  \item In algebra, we prove \textbf{equalities} directly.
  \item In analysis, we usually prove \textbf{inequalities} and we prove those
    inequalities by estimating.
\end{itemize}

% =============================================================================
\section{Basic set theory}
% =============================================================================

% ******************************
\subsection{Sets}
% ******************************

\textbf{Definition 0.3.1.} A \textit{set} is a collection of objects called
\textit{elements} or \textit{members}. A set with no objects is called the
\textit{empty set} and is denoted by $\emptyset$ (or sometimes by $\{\}$).

The \textbf{universe} is the set that contains only the elements that we are
interested in. It is generally understood from context and is not explicitly
mentioned.

The various set-related notations:
\begin{itemize}
  \item \textbf{Membership}:
    \begin{itemize}
      \item[$\bullet$] $a \in A$: the element $a$ belongs to the set $A$
      \item[$\bullet$] $a \notin A$: the element $a$ does not belong to the set
        $A$.
    \end{itemize}
  \item \textbf{Subset}:
    \begin{itemize}
      \item Used in this book: $A \subset B$ (at times: $B \supset A$)
      \item Alternatively: Some people prefer to use $A \subseteq B$ to denote
        ``A is a subset of B''.
    \end{itemize}
  \item \textbf{Equality}:
    \begin{itemize}
      \item[$\bullet$] $A = B$: A and B contain exactly the same elements.
      \item[$\bullet$] $A \neq B$
    \end{itemize}
  \item \textbf{Proper subset}:
    \begin{itemize}
      \item Used in this book: $A \subsetneq B$: $A \subset B$ and $A \neq B$.
      \item Alternatively: Some people prefer to use $A \subset B$ to denote
        ``A is a proper subset of B''. Note this can be confused with the
        notation of ``subset'' so consistency of usage is important.
    \end{itemize}
  \item \textbf{Set building notation}: $\{x \in A: P(x)\}$ refers to a subset
    of the set $A$ containing all the elements of $A$ that satisfy the property
    $P(x)$.
  \item \textbf{Natural numbers}: $\mathbb{N} := \{1, 2, 3, \ldots \}$
  \item \textbf{Integers}: $\mathbb{Z} := \{0, -1, 1, -2, 2, \ldots \}$
  \item \textbf{Rational numbers}: $\mathbb{Q} := \{\frac{m}{n}: m,n \in
    \mathbb{Z}, n \neq 0 \}$
  \item \textbf{Real numbers}: $\mathbb{R}$
  \item \textbf{Union}: $A \cup B := \{x: x \in A \ or \ x \in B\}$
  \item \textbf{Intersection}: $A \cap B := \{x: x \in A \ and \ x \in B\}$
  \item \textbf{Complement}:
    \begin{itemize}
      \item $A \setminus B := \{x: x \in A \ and \ x \notin B\}$
      \item $B^c$: If the set $A$ can be understood from the context. Here ``c''
        is the first letter of the word ``complement'', not a set $c$.
    \end{itemize}
  \item \textbf{Disjoint}: $A$ and $B$ are said to be \textit{disjoint} if $A
    \cap B = \emptyset$.
  \item \textbf{Union of an infinite collection of sets}:
    \[
      \bigcup_{n=1}^{\infty} A_n := \{x: x \in A_i, \exists i \in \mathbb{N}\}
    \]
    Note the use of $\exists$: Because this is the union of the sets $A_i$,
    by definition, it means that for any element $x$ in the final union, $x$
    belongs to at least one of the sets $A_i$, but it may or may not belong to
    all of them. Therefore, when we describe the membership of $x$, we must
    express the meaning of ``may or may not''.
  \item \textbf{Intersection of an infinite collection of sets}:
    \[
      \bigcap_{n=1}^{\infty} A_n := \{x: x \in A_i, \forall i \in \mathbb{N}\}
    \]
    The use of $\forall$ means that any element $x$ in the final set belongs
    to all of the sets $A_i$.
  \item \textbf{Unions/Intersection of sets with two indices}:
    \[
      \bigcup_{n=1}^{\infty} \bigcup_{m=1}^{\infty} A_{n,m} =
      \bigcup_{n=1}^{\infty} \Bigl(\bigcup_{m=1}^{\infty} A_{n,m}\Bigr)
    \]
    \[
      \bigcap_{n=1}^{\infty} \bigcap_{m=1}^{\infty} A_{n,m} =
      \bigcap_{n=1}^{\infty} \Bigl(\bigcap_{m=1}^{\infty} A_{n,m}\Bigr)
    \]
  \item \textbf{A more general notation}:
    \[
      \bigcup_{\lambda \in I} A_{\lambda} :=
      \{x: x \in A_{\lambda}, \exists \lambda \in I\}
    \]
    \[
      \bigcap_{\lambda \in I} A_{\lambda} :=
      \{x: x \in A_{\lambda}, \forall \lambda \in I\}
    \]
\end{itemize}

\textbf{Theorem 0.3.5 (DeMorgan)}: Let $A$ be the \textit{universe} and $B, C$
the subsets of $A$. Then:

\begin{itemize}
  \item $(B \cup C)^c$ = $B^c \cap C^c$
  \item $(B \cap C)^c$ = $B^c \cup C^c$
\end{itemize}

or, more generally,

\begin{itemize}
  \item $A \setminus (B \cup C)$ = $(A \setminus B) \cap (A \setminus C)$
  \item $A \setminus (B \cap C)$ = $(A \setminus B) \cup (A \setminus C)$
\end{itemize}

% ******************************
\subsection{Induction}
% ******************************

% ------------------------------
\subsubsection*{Theorem 0.3.6: Principle of induction}
% ------------------------------

Let $P(n)$ be a statement depending on a natural number $n$. Suppose that:

\begin{enumerate}
  \item (basis statement) $P(1)$ is true.
  \item (induction step) If $P(n)$ is true, then $P(n+1)$ is true.
\end{enumerate}

Then $P(n)$ is true for all $n \in \mathbb{N}$.

The textbook [1] offers the following proof:

\begin{displayquote}
  Suppose $S$ is the set of natural numbers $m$ for which $P(m)$ is not true.
  Suppose $S$ is nonempty. Then $S$ has a least element by the well ordering
  property. Let us call $m$ the least element of S. We know $1 \notin S$ by
  assumption. So $m > 1$ and $m - 1$ is a natural number as well. Since $m$ is
  the least element of $S$, we know that $P(m-1)$ is true. But by the induction
  step we see that $P(m-1+1) = P(m)$ is true, contradicting the statement that
  $m \in S$. Therefore, $S$ is empty and $P(n)$ is true for all $n \in
  \mathbb{N}$.
\end{displayquote}

My notes on the proof:

\begin{itemize}
  \item The proof uses contradiction. Therefore, we need to suppose the opposite
    conclusion of the theorem is true. Because the conclusion of the theorem is
    ``$P(n)$ is true for \textbf{all} $n \in \mathbb{N}$'', the opposite
    conclusion is ``there exist some $m \in \mathbb{N}$ that $P(m)$ is false''.
    This is why the first sentence says ``... $m$ for which $P(m)$ is not true''
    and ``$S$ is nonempty'': $S$ must not be empty, because otherwise the
    original conclusion is true and it makes no sense to use proof by
    contradiction.
  \item Regarding $1 \notin S$: The basis statement is $P(1)$ is true; $S$ is
    the set of natural numbers $m$ where $P(m)$ is false. Therefore, if $1 \in
    S$, that means $P(1)$ is false, which contradicts with the conditions of
    the theorem to-be-proven. Note that ``proof by contradiction'' starts with
    the opposite \textbf{conclusion} of the original theorem but it still
    accepts all the conditions of the original theorem. In this case, ``proof
    by contradiction'' still accepts the condition that $P(1)$ is true.
\end{itemize}

% ------------------------------
\subsubsection*{Theorem 0.3.9: Principle of strong induction}
% ------------------------------

Let $P(n)$ be a statement depending on a natural number $n$. Suppose that:

\begin{enumerate}
  \item (basis statement) $P(1)$ is true.
  \item (induction step) If $P(k)$ is true for all $k = 1, 2, \ldots, n$, then
    $P(n+1)$ is true.
\end{enumerate}

Then $P(n)$ is true for all $n \in \mathbb{N}$.

The textbook leaves the proof of this theorem as an exercise, so here is mine:

My proof: We still use the method of ``proof by contradiction''. Suppose $S$ is
the set of natural numbers $i$ for which $P(i)$ is not true and $S$ is not
empty. By the well ordering property, we know $S$ has a least element and let's
call it $m$. Because $P(k)$ is true for all $k = 1, 2, \ldots, n$, we know that
$1, 2, \ldots, n \notin S$. Therefore, $m > n$ and $m-1$ is a natural number,
too. Since $m$ is the least element of $S$, we know $m-1 \notin S$. Because
$P(i)$ is not true for all $i \in S$ and because $m-1 \notin S$, we know
$P(m-1)$ is true. However, by the induction step, we see that $P(m-1+1) = P(m)$
must be true, so $m \notin S$, contradicting the statement that $m \in S$.
Therefore, $S$ must be empty and $P(n)$ is true for all $n \in \mathbb{N}$.

% ******************************
\subsection{Functions}
% ******************************

In order to define functions rigorously, we must define the Cartesian product
firstly.

% ------------------------------
\subsubsection*{Definition 0.3.10 Cartesian product}
% ------------------------------

Let $A$ and $B$ be sets. The \textit{Cartesian product} is the set of tuples
defined as \[ A \times B := \{(x, y): x \in A, y \in B \} \].

\textbf{Note}: ``tuple'' is the same as the ``list'' as we see in ``Linear
Algebra Done Right''.

Examples:
\begin{itemize}
  \item $[0,1] \times [0,1]$ = $\{(0,0), (0,1), (1,0), (1,1)\}$
  \item $[0,1] \times [0,1]$ is also denoted as $[0,1]^2$.
  \item $\mathbb{R}^2$ = $\mathbb{R} \times \mathbb{R}$
\end{itemize}

% ------------------------------
\subsubsection*{Definition 0.3.11 Function}
% ------------------------------

A \textit{function} $f: A \rightarrow B$ is a subset $f$ of $A \times B$ such
that for each $x \in A$, there is a \textbf{unique} $(x,y) \in f$. We then
write $f(x) = y$.

The various terms that are related with functions:
\begin{itemize}
  \item Sometimes $f$ is called a \textbf{mapping} or a \textbf{map}: $f$
    \textbf{maps} $A$ to $B$.
  \item Sometimes the set $f$ is called the \textbf{graph} of the function
    rather than the function itself.
  \item \textbf{domain}: The set $A$ is called the domain of $f$. Sometimes it
    is (confusingly) denoted as $D(f)$.
  \item \textbf{range}: The set $R(f) := \{y \in B: \exists x: f(x) = y\}$ is
    called the range of $f$.
\end{itemize}

% ------------------------------
\subsubsection*{Definition 0.3.13 Direct image and inverse image}
% ------------------------------

Consider a function $f: A \rightarrow B$ and $C \subset A$. Define the
\textit{image} (or \textit{direct image}) of $C$ as \[ f(C) := \{f(x) \in B:
x \in C\} \].

Let $D \subset B$. Define the \textit{inverse image} of $D$ as \[ f^{-1}(D) :=
\{x \in A: f(x) \in D\}\].

\textbf{Note} the definition of inverse image: the elements in $D$ do not have
to have an element in $A$ that maps to it. See the example $f^{-1}(\{a,b,c\})$
in \textbf{Figure 3} in the textbook.

% ------------------------------
\subsubsection*{Proposition 0.3.15}
% ------------------------------

Consider $f: A \rightarrow B$. Let $C$, $D$ be subsets of $B$. Then:
\begin{enumerate}
  \item $f^{-1}(C \cup D)$ = $f^{-1}(C) \cup f^{-1}(D)$
  \item $f^{-1}(C \cap D)$ = $f^{-1}(C) \cap f^{-1}(D)$
  \item $f^{-1}(C^c)$ = $\bigl(f^{-1}(C)\bigr)^c$ (which means $f^{-1}(B
    \setminus C) = A \setminus f^{-1}(C)$)
\end{enumerate}

The textbook offers the proof for the first statement, but I want to prove it
with more details.

\textbf{My proof}:

To prove that two sets are equal, we need to use the definition of \textit{
equal} in definition 0.3.2, that two sets $A$ and $B$ are equal if $A \subset B$
and $B \subset A$.

\begin{enumerate}
  \item The proof is divided into three steps:
    \begin{enumerate}
      \item $\forall x \in f^{-1}(C \cup D)$, according to the definition of
        $f^{-1}$, we know $f(x) \in C \cup D$. According to the definition of
        \textit{union}, we know this means $f(x) \in C$ or $f(x) \in D$. When
        $f(x) \in C$, this means $x \in f^{-1}(C)$; when $f(x) \in D$, this
        means $x \in f^{-1}(D)$. According to the definition of \textit{union}
        again, we know this means $x \in f^{-1}(C) \cup f^{-1}(D)$. Therefore,
        the whole reasoning chain can be summarized as $\forall x \in f^{-1}(C
        \cup D) \Rightarrow x \in f^{-1}(C) \cup f^{-1}(D)$. According to the
        definition of \textit{subset}, this means $f^{-1}(C \cup D) \subset
        f^{-1}(C) \cup f^{-1}(D)$.
      \item $\forall x \in f^{-1}(C) \cup f^{-1}(D)$ means $x \in f^{-1}(C)$ or
        $x \in f^{-1}(D)$ which means $f(x) \in C$ or $f(x) \in D$ which means
        $f(x) \in C \cup D$. According to the definition of \textit{inverse
        image}, this means $x \in f^{-1}(C \cup D)$. Therefore, the whole
        reasoning chain can be summarized as $\forall x \in f^{-1}(C) \cup
        f^{-1}(D) \Rightarrow x \in f^{-1}(C \cup D)$. According to the
        definition of \textit{subset}, this means $f^{-1}(C) \cup f^{-1}(D)
        \subset f^{-1}(C \cup D)$.
      \item According to the definition of \textit{equal}, we know $f^{-1}(C
        \cup D)$ = $f^{-1}(C) \cup f^{-1}(D)$.
    \end{enumerate}
  \item The proof is divided into three steps:
    \begin{enumerate}
      \item $\forall x \in f^{-1}(C \cap D)$, according to the definition of
        $f^{-1}$, we know $f(x) \in C \cap D$. According to the definition of
        \textit{intersection}, we know this means $f(x) \in C$ and $f(x) \in D$.
        When $f(x) \in C$, this means $x \in f^{-1}(C)$; when $f(x) \in D$, this
        means $x \in f^{-1}(D)$. According to the definition of \textit{
        intersection} again, we know this means $x \in f^{-1}(C) \cap
        f^{-1}(D)$. Therefore, the whole reasoning chain can be summarized as
        $\forall x \in f^{-1}(C \cap D) \Rightarrow x \in f^{-1}(C) \cap
        f^{-1}(D)$. According to the definition of \textit{subset}, this means
        $f^{-1}(C \cap D) \subset f^{-1}(C) \cap f^{-1}(D)$.
      \item $\forall x \in f^{-1}(C) \cap f^{-1}(D)$ means $x \in f^{-1}(C)$ and
        $x \in f^{-1}(D)$ which means $f(x) \in C$ and $f(x) \in D$ which means
        $f(x) \in C \cap D$. According to the definition of \textit{inverse
        image}, this means $x \in f^{-1}(C \cap D)$. Therefore, the whole
        reasoning chain can be summarized as $\forall x \in f^{-1}(C) \cap
        f^{-1}(D) \Rightarrow x \in f^{-1}(C \cap D)$. According to the
        definition of \textit{subset}, this means $f^{-1}(C) \cap f^{-1}(D)
        \subset f^{-1}(C \cap D)$.
      \item According to the definition of \textit{equal}, we know $f^{-1}(C
        \cap D)$ = $f^{-1}(C) \cap f^{-1}(D)$.
    \end{enumerate}
  \item The proof is divided into three steps:
    \begin{enumerate}
      \item First of all, according to the definition of \textit{inverse image}
        on $f: A \rightarrow B$, we know that $\forall x \in f^{-1}(B \setminus
        C)$ comes to two conclusions:
        \begin{enumerate}
          \item $x \in A$
          \item $f(x) \in B \setminus C$
        \end{enumerate}
        The second conclusion means $f(x) \in B$ and $f(x) \notin C$. When $f(x)
        \notin C$, we know $x \notin f^{-1}(C)$ (because if $x \in f^{-1}(C)$,
        by definition it means $f(x) \in C$, contradicting with the condition
        that $f(x) \notin C$). Therefore, now we have the following two
        conditions hold at the same time:
        \begin{enumerate}
          \item $x \in A$
          \item $x \notin f^{-1}(C)$
        \end{enumerate}
        This means $x \in A \setminus f^{-1}(C)$. The whole reasoning chain is
        \[
          \forall x \in f^{-1}(B \setminus C) \Rightarrow x \in A \setminus
          f^{-1}(C)
        \]
        So we know $f^{-1}(B \setminus C) \subset (A \setminus f^{-1}(C))$.
      \item Secondly, $\forall x \in A \setminus f^{-1}(C)$, we come to two
        conclusions:
        \begin{enumerate}
          \item $x \in A \Rightarrow f(x) \in B$.
          \item $x \notin f^{-1}(C) \Rightarrow f(x) \notin C$.
        \end{enumerate}
        Therefore, we know $f(x) \in (B \setminus C)$, so $x \in f^{-1}(B
          \setminus C)$. The whole
        reasoning chain is
        \[
          \forall x \in A \setminus f^{-1}(C) \Rightarrow x \in f^{-1}(B
          \setminus C)
        \]
        So we know $A \setminus f^{-1}(C) \subset f^{-1}(B \setminus C)$
      \item According to the definition of \textit{equal}, we know $f^{-1}(B
        \setminus C)$ = $A \setminus f^{-1}(C)$.
    \end{enumerate}
\end{enumerate}

% ------------------------------
\subsubsection*{Proposition 0.3.16}
% ------------------------------

Consider $f: A \rightarrow B$. Let $C$, $D$ be subsets of $A$. Then
\begin{enumerate}
  \item $f(C \cup D)$ = $f(C) \cup f(D)$
  \item $f(C \cap D) \subset f(C) \cap f(D)$
\end{enumerate}

To prove 1, we need to use the following conclusion: Given $f: A \rightarrow B$.
Let $C$, $D$ be subsets of $A$. Then \[f(x) \in f(C) \cup f(D) \Rightarrow
x \in C \cup D\]

We can use contradiction to prove this. Suppose $\exists u \notin (C \cup D)$
such that $f(u) \in f(C) \cup f(D)$. Because $C$ and $D$ are discussed under
the universe $A$, we have $u \notin (C \cup D)$, which means $u \in A \setminus
(C \cup D)$, which means $u \in (A \setminus C)$ AND $u \in (A \setminus D)$,
which means $u \notin C$ AND $u \notin D$.

When $u \notin C$, we can tell that $f(u) \notin f(C)$ (because otherwise if
$f(u) \in f(C)$, according to the definition of \textit{direct image}, $u$ must
be an element of $C$, contradicting the precondition $u \notin C$). Similarly,
we can tell that when $u \notin D$, $f(u) \notin f(D)$.

Because $\forall x \in A$, we have $f(x) \in B$, so $f(C)$ and $f(D)$ must be
subsets of $B$, i.e., $B$ is the universe of $C$ and $D$. Therefore, when we
say $f(u) \notin f(C)$, we mean $f(u) \in B \setminus f(C)$; when we say $f(u)
\notin f(D)$, we mean $f(u) \in B \setminus f(D)$. Because $f(u) \notin f(C)$
AND $f(u) \notin f(D)$, we have $f(u) \in \bigl(B \setminus f(C)\bigr) \cap
\bigl(B \setminus f(D)\bigr) = B \setminus \bigl(f(C) \cup f(D)\bigr)$, so
$f(u) \in B$ but $f(u) \notin \bigl(f(C) \cup f(D)\bigr)$ which contradicts
the precondition that $f(u) \in \bigl(f(C) \cup f(D)\bigr)$. So such a $u
\notin (C \cup D)$ does \textbf{not} exist.

\textbf{My proof of 1}:

To prove $f(C \cup D)$ = $f(C) \cup f(D)$, we need to prove $f(C \cup D)
\subset f(C) \cup f(D)$ and $f(C \cup D) \supset f(C) \cup f(D)$.

According to the definition of \textit{direct image}, $f(C \cup D) := \{f(x)
\in B: x \in C \cup D\}$, so $\forall f(x) \in f(C \cup D)$, we have $x \in C
\cup D$, so $x \in C$ or $x \in D$. When $x \in C$, $f(x) \in f(C) := \{f(x): x
\in C\}$; when $x \in D$, $f(x) \in f(D) := \{f(x): x \in D\}$. Therefore, $f(x)
\in f(C)$ or $f(x) \in f(D)$ depending on $x \in C$ or $x \in D$, i.e., when $x
\in C \cup D$, $f(x) \in B$, so we know all the $f(x)$ when $x \in C \cup D$ is
defined as $f(C \cup D)$. So $\forall f(x) \in f(C) \cup f(D)$, we have $f(x)
\in f(C \cup D)$. So $f(C \cup D) \subset f(C \cup D)$.

On the other way, $\forall f(x) \in f(C) \cup f(D)$ $\Rightarrow$ $f(x) \in
f(C)$ or $f(x) \in f(D)$. According to the definition of \textit{direct image},
\begin{itemize}
  \item $f(C) := {f(x) \in B: x \in C}$
  \item $f(D) := {f(x) \in B: x \in D}$.
\end{itemize}

Therefore:
\begin{itemize}
  \item When $f(x) \in f(C)$, we know $x \in C$.
  \item When $f(x) \in f(D)$, we know $x \in D$.
\end{itemize}

Therefore, when $f(x) \in f(C) \cup f(D)$, we have $x \in C$ or $x \in D$, i.e.,
$x \in C \cup D$. According to the definition of \textit{direct image}, when $x
\in C \cup D$, $f(x)$ is defined as $f(C \cup D)$. So we know $f(x) \in f(C
\cup D)$. So $\forall f(x) \in f(C) \cup f(D)$, we have $f(x) \in f(C \cup D)$.
So $f(C \cup D) \subset f(C \cup D)$.

To sum up, we have $f(C \cup D) \subset f(C) \cup f(D)$ and $f(C \cup D)
\supset f(C) \cup f(D)$, so $f(C \cup D)$ = $f(C) \cup f(D)$.

\textbf{My proof of 2}:

According to the definition of \textit{direct image}, $f(C \cap D) := \{f(x)
\in B: x \in C \cap D\}$, so $\forall f(x) \in f(C \cap D)$, we have $x \in C
\cap D$, so $x \in C$ and $x \in D$.

\begin{itemize}
  \item When $x \in C$, we have $f(x) \in f(C)$.
  \item When $x \in D$, we have $f(x) \in f(D)$.
\end{itemize}

Because $x \in C$ and $x \in D$, we have $f(x) \in f(C)$ and $f(x) \in f(D)$,
namely $f(x) \in f(C) \cap f(D)$.

In sum, we have $\forall f(x) \in f(C \cap D)$, $f(x) \in f(C) \cap f(D)$, so
we have $f(C \cap D) \subset f(C) \cap f(D)$.

\textbf{The other way may not hold}, i.e., $f(C) \cap f(D)$ may \textbf{not} be
a subset of $f(C \cap D)$. A counter example is $f: x \rightarrow x^2, x \in
\mathbb{R}$. Here, in the context of this proposition, $A$ and $B$ are both
$\mathbb{R}$. Now let $C := [-2, 0]$ and $D := [0, 2]$. We have:

\begin{itemize}
  \item $f(C) = [0, 4]$
  \item $f(D) = [0, 4]$
  \item $f(C) \cap f(D) = [0, 4]$
  \item $C \cap D = \{0\}$, so $f(C \cap D) = f(\{0\}) = [0]$
\end{itemize}

Obviously, $f(C) \cap f(D)$ is \textbf{not} a subset of $f(C \cap D)$.

% =============================================================================
%
% Chapter 1: Real Numbers
%
% =============================================================================

\chapter{Real Numbers}

TODO

\chapter*{References}
\addcontentsline{toc}{chapter}{References}

\begin{itemize}
  \item $[1]$ \href{https://ocw.mit.edu/courses/18-100a-real-analysis-fall-2020/resources/mit18_100af20_basic_analysis/}{Lebl, Jiří: \it{Basic Analysis I: Introduction to Real Analysis, Volume 1}}
\end{itemize}

\end{document}
